chore: undo necessary changes

SSA/Projects/CIRCT/Handshake-to-DC/ForkData.lean
@@ -1,13 +1,8 @@
+import SSA.Projects.CIRCT.DC.DC
 import SSA.Projects.CIRCT.Handshake.Handshake
-import SSA.Projects.CIRCT.DCxComb.DCxCombFunctor
 import SSA.Projects.CIRCT.Stream.Stream
 import SSA.Projects.CIRCT.Stream.WeakBisim
 import SSA.Core.Tactic
-import SSA.Core.ErasedContext
-import SSA.Core.HVector
-import SSA.Core.EffectKind
-import SSA.Core.Util
-
 
 namespace CIRCTStream
 namespace Stream.Bisim
@@ -38,8 +33,8 @@ theorem EqIsBisim {α} : @IsBisim α Eq := by
   and_intros; all_goals first | rfl | intros _ h; cases h
 
 theorem fork_hs_dc_equiv_fst (x : DCOp.TokenStream):
-    (DCOp.fork (x)).fst ~ (HandshakeOp.fork (x)).fst := by
-  simp [Bisim, DCOp.fork, HandshakeOp.fork]
+    (DCOp.fork (x)).fst ~ (Handshake.fork (x)).fst := by
+  simp [Bisim, DCOp.fork, Handshake.fork]
   exists Eq
   and_intros
   · rw [corec₂_eq_tok]
@@ -47,8 +42,8 @@ theorem fork_hs_dc_equiv_fst (x : DCOp.TokenStream):
   · apply EqIsBisim
 
 theorem fork_hs_dc_equiv_snd (x : DCOp.TokenStream):
-    (DCOp.fork (x)).snd ~ (HandshakeOp.fork (x)).snd := by
-  simp [Bisim, DCOp.fork, HandshakeOp.fork]
+    (DCOp.fork (x)).snd ~ (Handshake.fork (x)).snd := by
+  simp [Bisim, DCOp.fork, Handshake.fork]
   exists Eq
   and_intros
   · rw [corec₂_eq_tok]
@@ -60,39 +55,36 @@ theorem fork_hs_dc_equiv_snd (x : DCOp.TokenStream):
 
 /- step 1: write dc circuit -/
 
-open MLIR AST in
-
-
-
 unseal String.splitOnAux in
-def DCxCombFork := [DCxComb_com| {
-  ^entry(%0 : !ValueStream_8):
-    %unpack12 = "DCxComb.unpack" (%0) : (!ValueStream_8) -> (!ValueTokenStream_8)
-    %unpack1 = "DCxComb.fstVal" (%unpack12) : (!ValueTokenStream_8) -> (!ValueStream_8)
-    %unpack2 = "DCxComb.sndVal" (%unpack12) : (!ValueTokenStream_8) -> (!TokenStream)
-    %fork12 = "DCxComb.fork" (%unpack2) : (!TokenStream) -> (!TokenStream2)
-    %fork1 = "DCxComb.fst" (%fork12) : (!TokenStream2) -> (!TokenStream)
-    %fork2 = "DCxComb.snd" (%fork12) : (!TokenStream2) -> (!TokenStream)
-    %pack1 = "DCxComb.pack" (%unpack1, %fork1) : (!ValueStream_8, !TokenStream) -> (!ValueStream_8)
-    %pack2 = "DCxComb.pack" (%unpack1, %fork2) : (!ValueStream_8, !TokenStream) -> (!ValueStream_8)
-    %pack12 = "DCxComb.pair" (%pack1, %pack2) : (!ValueStream_8, !ValueStream_8) -> (!ValueStream2_8)
-    "return" (%pack12) : (!ValueStream2_8) -> ()
+def DCFork := [DC_com| {
+  ^entry(%0 : !ValueStream_Int):
+    %unpack12 = "DC.unpack" (%0) : (!ValueStream_Int) -> (!ValueTokenStream_Int)
+    %unpack1 = "DC.fstVal" (%unpack12) : (!ValueTokenStream_Int) -> (!ValueStream_Int)
+    %unpack2 = "DC.sndVal" (%unpack12) : (!ValueTokenStream_Int) -> (!TokenStream)
+    %fork12 = "DC.fork" (%unpack2) : (!TokenStream) -> (!TokenStream2)
+    %fork1 = "DC.fst" (%fork12) : (!TokenStream2) -> (!TokenStream)
+    %fork2 = "DC.snd" (%fork12) : (!TokenStream2) -> (!TokenStream)
+    %pack1 = "DC.pack" (%unpack1, %fork1) : (!ValueStream_Int, !TokenStream) -> (!ValueStream_Int)
+    %pack2 = "DC.pack" (%unpack1, %fork2) : (!ValueStream_Int, !TokenStream) -> (!ValueStream_Int)
+    %pack12 = "DC.pair" (%pack1, %pack2) : (!ValueStream_Int, !ValueStream_Int) -> (!ValueStream2_Int)
+    "return" (%pack12) : (!ValueStream2_Int) -> ()
   }]
+
 /- step 2: denote dc circuit -/
 
-#check DCxCombFork
-#eval DCxCombFork
-#reduce DCxCombFork
-#check DCxCombFork.denote
-#print axioms DCxCombFork
+#check DCFork
+#eval DCFork
+#reduce DCFork
+#check DCFork.denote
+#print axioms DCFork
 
 def ofList (vals : List (Option α)) : Stream α :=
   fun i => (vals.get? i).join
 
-def x : DCOp.ValueStream (BitVec 8) := ofList [some 1, none, some 2, some 5, none]
+def x : DCOp.ValueStream Int := ofList [some 1, none, some 2, some 5, none]
 
-def test : CIRCTStream.DCOp.ValueStream (BitVec 8) × CIRCTStream.DCOp.ValueStream (BitVec 8)  :=
-  DCxCombFork.denote (Ctxt.Valuation.ofHVector (.cons x <| .nil))
+def test : DCOp.ValueStream Int × DCOp.ValueStream Int :=
+  DCFork.denote (Ctxt.Valuation.ofHVector (.cons x <| .nil))
 
 /- step 3: prove equivalence -/
 
@@ -120,20 +112,19 @@ theorem tail_iterate' {α} {n} {s : Stream' α} : Stream'.iterate Stream'.tail s
   tail_iterate''
 
 open Ctxt in
-theorem equiv_fork_fst (streamInt : DCOp.ValueStream (BitVec 8)) :
-  (HandshakeOp.fork streamInt).fst ~ (DCxCombFork.denote (Valuation.ofHVector (.cons streamInt <| .nil))).fst := by
-  simp [EffectKind.toMonad_impure, DCxCombFork,
+theorem equiv_fork_fst (streamInt : DCOp.ValueStream Int) :
+  (Handshake.fork streamInt).fst ~ (DCFork.denote (Valuation.ofHVector (.cons streamInt <| .nil))).fst := by
+  simp only [MLIR2DC.instDialectDenoteDC, EffectKind.toMonad_impure, DCFork,
     EffectKind.pure_sup_pure_eq, DerivedCtxt.ofCtxt, DerivedCtxt.snoc.eq_1, get?.eq_1,
     Var.zero_eq_last, zero_add, Var.succ_eq_toSnoc, Nat.reduceAdd, Valuation.ofHVector,
     Ctxt.ofList.eq_1, Com.denote_var, EffectKind.toMonad_pure, Com.denote_ret, Id.pure_eq,
     Id.bind_eq]
-  sorry
-  -- unfold HandshakeOp.fork DCOp.pack DCOp.unpack DCOp.fork
-  -- simp_peephole
-  -- unfold Bisim; exists Eq
-  -- rw [corec₂_corec1]
-  -- and_intros
-  -- · sorry
+  unfold Handshake.fork DCOp.pack DCOp.unpack DCOp.fork
+  simp_peephole
+  unfold Bisim; exists Eq
+  rw [corec₂_corec1]
+  and_intros
+  · sorry
     -- · intros a b hm
       -- and_intros
       -- all_goals
@@ -187,7 +178,7 @@ theorem equiv_fork_fst (streamInt : DCOp.ValueStream (BitVec 8)) :
     --     unfold Stream'.map Stream'.get
     --     dsimp only
     --     rw [tail_iterate']
-  -- · apply EqIsBisim
+  · apply EqIsBisim
 
 theorem stream_pair_1 (s : Stream α) (f : Stream α → Option α × Option α × Stream α):
     (corec₂ s f).1 = corec s (fun x => let ⟨f1, _, f2⟩ := f x; (f1, f2)) := by
@@ -206,10 +197,10 @@ def IsBisim' (R' : Stream α → Stream α → Prop) : Prop :=
     ∧ (∀ i < n, a.get i = none)
     ∧ (∀ j < m, b.get j = none)
 
-theorem corec₂_eq_corec_of_corec₂ (streamInt: DCOp.ValueStream (BitVec w)) :
+theorem corec₂_eq_corec_of_corec₂ (streamInt: DCOp.ValueStream Int) :
     (corec₂ streamInt fun x => (x 0, x 0, x.tail)).1 ≈
     corec
-      ((corec₂ streamInt fun (x : DCOp.ValueStream (BitVec w)) =>
+      ((corec₂ streamInt fun (x : DCOp.ValueStream Int) =>
             (match x 0 with
               | some val => (x 0, some (), x.tail)
               | none => (none, none, x.tail))).1,
