SSA/Projects/CIRCT/Handshake-to-DC/JoinPackUnpack.lean
@@ -1,5 +1,4 @@
-import SSA.Projects.CIRCT.DCxComb.DCxComb
-
+import SSA.Projects.CIRCT.DC.DC
 import SSA.Projects.CIRCT.Handshake.Handshake
 import SSA.Projects.CIRCT.Stream.Stream
 import SSA.Projects.CIRCT.Stream.WeakBisim
@@ -32,48 +31,30 @@ namespace Stream.Bisim
 
 -- also changed to return a single value, the third arg is not used anyways
 unseal String.splitOnAux in
-def joinPackUnpack := [DCxComb_com| {
-  ^entry(%0: !ValueStream_64, %1: !ValueStream_64):
-    -- // CHECK:           %[[VAL_3:.*]], %[[VAL_4:.*]] = dc.unpack %[[VAL_0]] : !dc.value<i64>
-    %unpack0 = "DCxComb.unpack" (%0) : (!ValueStream_64) -> (!ValueTokenStream_64)
-    %unpack0val = "DCxComb.fstVal" (%unpack0) : (!ValueTokenStream_64) -> (!ValueStream_64)
-    %unpack0tok = "DCxComb.sndVal" (%unpack0) : (!ValueTokenStream_64) -> (!TokenStream)
-    -- // CHECK:           %[[VAL_5:.*]], %[[VAL_6:.*]] = dc.unpack %[[VAL_1]] : !dc.value<i64>
-    %unpack1 = "DCxComb.unpack" (%1) : (!ValueStream_64) -> (!ValueTokenStream_64)
-    %unpack1val = "DCxComb.fstVal" (%unpack1) : (!ValueTokenStream_64) -> (!ValueStream_64)
-    %unpack1tok = "DCxComb.sndVal" (%unpack1) : (!ValueTokenStream_64) -> (!TokenStream)
-    -- // CHECK:           %[[VAL_7:.*]] = dc.join %[[VAL_3]], %[[VAL_5]]
-    %join01 = "DCxComb.join" (%unpack0tok, %unpack1tok) : (!TokenStream, !TokenStream) -> (!TokenStream)
+def joinPackUnpack := [DC_com| {
+  ^entry(%0: !ValueStream_Int, %1: !ValueStream_Int):
+    %unpack0 = "DC.unpack" (%0) : (!ValueStream_Int) -> (!ValueTokenStream_Int)
+    %unpack1 = "DC.unpack" (%1) : (!ValueStream_Int) -> (!ValueTokenStream_Int)
+    %unpack01 = "DC.fstVal" (%unpack0) : (!ValueTokenStream_Int) -> (!ValueStream_Int)
+    %unpack02 = "DC.sndVal" (%unpack0) : (!ValueTokenStream_Int) -> (!TokenStream)
+    %unpack11 = "DC.fstVal" (%unpack1) : (!ValueTokenStream_Int) -> (!ValueStream_Int)
+    %unpack12 = "DC.sndVal" (%unpack1) : (!ValueTokenStream_Int) -> (!TokenStream)
+    %join01 = "DC.join" (%unpack02, %unpack12) : (!TokenStream, !TokenStream) -> (!TokenStream)
+    -- here we have an `arith` operation whose result we should pack :
     -- // CHECK:           %[[VAL_8:.*]] = arith.cmpi slt, %[[VAL_4]], %[[VAL_6]] : i64
-    %readyVal0 = "DCxComb.popReady_100" (%unpack0val) : (!ValueStream_64) -> (i64)
-    %readyVal1 = "DCxComb.popReady_100" (%unpack1val) : (!ValueStream_64) -> (i64)
-    %slt = "DCxComb.icmp_slt" (%readyVal0, %readyVal1) : (i64, i64) -> (i1)
-    %sltStream = "DCxComb.pushReady_1" (%slt) : (i1) -> (!ValueStream_1)
-    -- // CHECK:           %[[VAL_9:.*]] = dc.pack %[[VAL_7]], %[[VAL_8]] : i1
-    %pack = "DCxComb.pack" (%sltStream, %join01) : (!ValueStream_1, !TokenStream) -> (!ValueStream_1)
-    -- // CHECK:           %[[VAL_10:.*]], %[[VAL_11:.*]] = dc.unpack %[[VAL_9]] : !dc.value<i1>
-    %unpackP = "DCxComb.unpack" (%pack) : (!ValueStream_1) -> (!ValueTokenStream_1)
-    %unpackPval = "DCxComb.fstVal" (%unpackP) : (!ValueTokenStream_1) -> (!ValueStream_1)
-    %unpackPtok = "DCxComb.sndVal" (%unpackP) : (!ValueTokenStream_1) -> (!TokenStream)
-    -- // CHECK:           %[[VAL_12:.*]], %[[VAL_13:.*]] = dc.unpack %[[VAL_1]] : !dc.value<i64>
-    %unpackBis0 = "DCxComb.unpack" (%0) : (!ValueStream_64) -> (!ValueTokenStream_64)
-    %unpackBis0val = "DCxComb.fstVal" (%unpackBis0) : (!ValueTokenStream_64) -> (!ValueStream_64)
-    %unpackBis0tok = "DCxComb.sndVal" (%unpackBis0) : (!ValueTokenStream_64) -> (!TokenStream)
-    -- // CHECK:           %[[VAL_14:.*]], %[[VAL_15:.*]] = dc.unpack %[[VAL_0]] : !dc.value<i64>
-    %unpackBis1 = "DCxComb.unpack" (%1) : (!ValueStream_64) -> (!ValueTokenStream_64)
-    %unpackBis1val = "DCxComb.fstVal" (%unpackBis1) : (!ValueTokenStream_64) -> (!ValueStream_64)
-    %unpackBis1tok = "DCxComb.sndVal" (%unpackBis1) : (!ValueTokenStream_64) -> (!TokenStream)
-    -- // CHECK:           %[[VAL_16:.*]] = dc.join %[[VAL_10]], %[[VAL_12]], %[[VAL_14]]]
-    %joinPackBis = "DCxComb.join" (%unpackPtok, %unpackBis0tok, %unpackBis1tok) : (!TokenStream, !TokenStream, !TokenStream) -> (!TokenStream)
-    -- // CHECK:           %[[VAL_17:.*]] = arith.select %[[VAL_11]], %[[VAL_13]], %[[VAL_15]] : i64
-    %readyValP = "DCxComb.popReady_100" (%unpackPval) : (!ValueStream_1) -> (i1)
-    %readyValBis0 = "DCxComb.popReady_100" (%unpackBis0val) : (!ValueStream_64) -> (i64)
-    %readyValBis1 = "DCxComb.popReady_100" (%unpackBis1val) : (!ValueStream_64) -> (i64)
-    %muxOut = "DCxComb.mux" (%readyValBis0, %readyValBis1, %readyValP) : (i64, i64, i1) -> (i64)
-    -- // CHECK:           %[[VAL_18:.*]] = dc.pack %[[VAL_16]], %[[VAL_17]] : i64
-    -- %streamVal = "DCxComb.pushReady_64" (%muxOut) : (i64) -> (!ValueStream_64)
-    -- %packBis = "DCxComb.pack" (%muxOut, %joinPackBis) : (!ValueStream_64, !TokenStream) -> (!ValueStream_64)
-    "return" (%0) : (!ValueStream_64) -> ()
+    -- instead, I am packing `%unpack01`, for the time being
+    %pack = "DC.pack" (%unpack01, %join01) : (!ValueStream_Int, !TokenStream) -> (!ValueStream_Int)
+    %unpackPack = "DC.unpack" (%pack) : (!ValueStream_Int) -> (!ValueTokenStream_Int)
+    %unpack0Pack1 = "DC.fstVal" (%unpackPack) : (!ValueTokenStream_Int) -> (!ValueStream_Int)
+    %unpack0Pack2 = "DC.sndVal" (%unpackPack) : (!ValueTokenStream_Int) -> (!TokenStream)
+    %unpack0Bis = "DC.unpack" (%0) : (!ValueStream_Int) -> (!ValueTokenStream_Int)
+    %unpack0Bis1 = "DC.fstVal" (%unpack0Bis) : (!ValueTokenStream_Int) -> (!ValueStream_Int)
+    %unpack0Bis2 = "DC.sndVal" (%unpack0Bis) : (!ValueTokenStream_Int) -> (!TokenStream)
+    -- we currently don't support n-ary joins so will keep it binary for now
+    %joinPackBis = "DC.join" (%unpack0Bis2, %unpack0Pack2) : (!TokenStream, !TokenStream) -> (!TokenStream)
+    -- again avoiding `arith` operation
+    %packBis = "DC.pack" (%unpack0Bis1, %joinPackBis) : (!ValueStream_Int, !TokenStream) -> (!ValueStream_Int)
+    "return" (%packBis) : (!ValueStream_Int) -> ()
   }]
 
 #check joinPackUnpack
